Standardizing SMACK names. * Every identifier introduced by smack now begins with '$'. * Short identifiers are preferred, when possible. * Functions are preferred to procedures for arithmetic predicates. Also, using std namespace, and std::endl, uniformly.

include/BplPrintUtils.h
@@ -24,7 +24,7 @@ private:
 public:
   printVarDecl(std::ostream &stream, std::string varTypeP) : os(stream), varType(varTypeP) {}
   void operator()(std::string var) {
-    os << "var " << var << " : " << varType << ";\n";
+    os << "var " << var << " : " << varType << ";" << std::endl;
   }
 };
 
